rt ainvs: proof update for domain_time fix
Signed-off-by: Michael McInerney <m.mcinerney@unsw.edu.au>

proof/invariant-abstract/DetSchedDomainTime_AI.thy
@@ -15,7 +15,8 @@ text \<open>
 
 (* Note: domains in the domain list should also be \<le> maxDomain, but this is not needed right now *)
 definition
-  "valid_domain_list_2 dlist \<equiv> 0 < length dlist \<and> (\<forall>(d,time) \<in> set dlist. 0 < time)"
+  "valid_domain_list_2 dlist
+     \<equiv> 0 < length dlist \<and> (\<forall>(d,time) \<in> set dlist. 0 < us_to_ticks (time * \<mu>s_to_ms))"
 
 abbreviation
   valid_domain_list :: "'z state \<Rightarrow> bool"
@@ -64,50 +65,42 @@ locale DetSchedDomainTime_AI =
     "\<And>P t f. \<lbrace>\<lambda>s::det_state. P (domain_list s)\<rbrace> handle_vm_fault t f \<lbrace>\<lambda>_ s. P (domain_list s)\<rbrace>"
   assumes prepare_thread_delete_domain_list_inv'[wp]:
     "\<And>P t. \<lbrace>\<lambda>s::det_state. P (domain_list s)\<rbrace> prepare_thread_delete t \<lbrace>\<lambda>_ s. P (domain_list s)\<rbrace>"
-  assumes finalise_cap_domain_time_inv'[wp]:
-    "\<And>P cap fin. \<lbrace>\<lambda>s::det_state. P (domain_time s)\<rbrace> arch_finalise_cap cap fin \<lbrace>\<lambda>_ s. P (domain_time s)\<rbrace>"
-  assumes arch_activate_idle_thread_domain_time_inv'[wp]:
-    "\<And>P t. \<lbrace>\<lambda>s::det_state. P (domain_time s)\<rbrace> arch_activate_idle_thread t \<lbrace>\<lambda>_ s. P (domain_time s)\<rbrace>"
-  assumes arch_switch_to_thread_domain_time_inv'[wp]:
-    "\<And>P t. \<lbrace>\<lambda>s::det_state. P (domain_time s)\<rbrace> arch_switch_to_thread t \<lbrace>\<lambda>_ s. P (domain_time s)\<rbrace>"
-  assumes arch_switch_to_thread_domain_consumed_time_inv'[wp]:
-    "\<And>P t. \<lbrace>\<lambda>s::det_state. P (domain_time s)(consumed_time s)\<rbrace> arch_switch_to_thread t \<lbrace>\<lambda>_ s. P (domain_time s)(consumed_time s)\<rbrace>"
-  assumes arch_get_sanitise_register_info_domain_time_inv'[wp]:
-    "\<And>P t. \<lbrace>\<lambda>s::det_state. P (domain_time s)\<rbrace> arch_get_sanitise_register_info t \<lbrace>\<lambda>_ s. P (domain_time s)\<rbrace>"
-  assumes arch_switch_to_idle_thread_domain_time_inv'[wp]:
-    "\<And>P. \<lbrace>\<lambda>s::det_state. P (domain_time s)\<rbrace> arch_switch_to_idle_thread \<lbrace>\<lambda>_ s. P (domain_time s)\<rbrace>"
-  assumes arch_switch_to_idle_thread_domain_consumed_time_inv'[wp]:
-    "\<And>P. \<lbrace>\<lambda>s::det_state. P (domain_time s)(consumed_time s)\<rbrace> arch_switch_to_idle_thread \<lbrace>\<lambda>_ s. P (domain_time s)(consumed_time s)\<rbrace>"
-  assumes handle_arch_fault_reply_domain_time_inv'[wp]:
-    "\<And>P f t x y. \<lbrace>\<lambda>s::det_state. P (domain_time s)\<rbrace> handle_arch_fault_reply f t x y \<lbrace>\<lambda>_ s. P (domain_time s)\<rbrace>"
-  assumes init_arch_objects_domain_time_inv'[wp]:
-    "\<And>P t p n s r. \<lbrace>\<lambda>s::det_state. P (domain_time s)\<rbrace> init_arch_objects t p n s r \<lbrace>\<lambda>_ s. P (domain_time s)\<rbrace>"
-  assumes arch_post_modify_registers_domain_time_inv'[wp]:
-    "\<And>P t p. \<lbrace>\<lambda>s::det_state. P (domain_time s)\<rbrace> arch_post_modify_registers t p \<lbrace>\<lambda>_ s. P (domain_time s)\<rbrace>"
-  assumes arch_invoke_irq_control_domain_time_inv'[wp]:
-    "\<And>P i. \<lbrace>\<lambda>s::det_state. P (domain_time s)\<rbrace> arch_invoke_irq_control i \<lbrace>\<lambda>_ s. P (domain_time s)\<rbrace>"
-  assumes handle_vm_fault_domain_time_inv'[wp]:
-    "\<And>P t f. \<lbrace>\<lambda>s::det_state. P (domain_time s)\<rbrace> handle_vm_fault t f \<lbrace>\<lambda>_ s. P (domain_time s)\<rbrace>"
-  assumes prepare_thread_delete_domain_time_inv'[wp]:
-    "\<And>P t. \<lbrace>\<lambda>s::det_state. P (domain_time s)\<rbrace> prepare_thread_delete t \<lbrace>\<lambda>_ s. P (domain_time s)\<rbrace>"
-  assumes make_arch_fault_msg_domain_time_inv'[wp]:
-    "\<And>P ft t. \<lbrace>\<lambda>s::det_state. P (domain_time s)\<rbrace> make_arch_fault_msg ft t \<lbrace>\<lambda>_ s. P (domain_time s)\<rbrace>"
+  assumes finalise_cap_domain_time_scheduler_action_inv'[wp]:
+    "\<And>P cap fin. arch_finalise_cap cap fin \<lbrace>\<lambda>s :: det_state. P (domain_time s) (scheduler_action s)\<rbrace>"
+  assumes arch_activate_idle_thread_domain_time_schedule_action_inv'[wp]:
+    "\<And>P t. arch_activate_idle_thread t \<lbrace>\<lambda>s :: det_state. P (domain_time s) (scheduler_action s)\<rbrace>"
+  assumes arch_switch_to_thread_domain_scheduler_action_inv'[wp]:
+    "\<And>P t. arch_switch_to_thread t \<lbrace>\<lambda>s :: det_state. P (domain_time s) (scheduler_action s)\<rbrace>"
+  assumes arch_get_sanitise_register_info_domain_time_scheduler_actioninv'[wp]:
+    "\<And>P t. arch_get_sanitise_register_info t \<lbrace>\<lambda>s :: det_state. P (domain_time s) (scheduler_action s)\<rbrace>"
+  assumes arch_switch_to_idle_thread_domain_time_scheduler_action_inv'[wp]:
+    "\<And>P. arch_switch_to_idle_thread \<lbrace>\<lambda>s :: det_state. P (domain_time s) (scheduler_action s)\<rbrace>"
+  assumes arch_switch_to_idle_thread_domain_scheduler_action_inv'[wp]:
+    "\<And>P. arch_switch_to_idle_thread \<lbrace>\<lambda>s :: det_state. P (domain_time s) (scheduler_action s)\<rbrace>"
+  assumes handle_arch_fault_reply_domain_time_scheduler_action_inv'[wp]:
+    "\<And>P f t x y. handle_arch_fault_reply f t x y \<lbrace>\<lambda>s :: det_state. P (domain_time s) (scheduler_action s)\<rbrace>"
+  assumes init_arch_objects_domain_time_scheduler_action_inv'[wp]:
+    "\<And>P t p n s r. init_arch_objects t p n s r \<lbrace>\<lambda>s :: det_state. P (domain_time s) (scheduler_action s)\<rbrace>"
+  assumes arch_post_modify_registers_domain_time_scheduler_action_inv'[wp]:
+    "\<And>P t p. arch_post_modify_registers t p \<lbrace>\<lambda>s :: det_state. P (domain_time s) (scheduler_action s)\<rbrace>"
+  assumes arch_invoke_irq_control_domain_time_scheduler_action_inv'[wp]:
+    "\<And>P i. arch_invoke_irq_control i \<lbrace>\<lambda>s :: det_state. P (domain_time s) (scheduler_action s)\<rbrace>"
+  assumes handle_vm_fault_domain_time_scheduler_action_inv'[wp]:
+    "\<And>P t f. handle_vm_fault t f \<lbrace>\<lambda>s :: det_state. P (domain_time s) (scheduler_action s)\<rbrace>"
+  assumes prepare_thread_delete_domain_time_scheduler_action_inv'[wp]:
+    "\<And>P t. prepare_thread_delete t \<lbrace>\<lambda>s :: det_state. P (domain_time s) (scheduler_action s)\<rbrace>"
+  assumes make_arch_fault_msg_domain_time_scheduler_action_inv'[wp]:
+    "\<And>P ft t. make_arch_fault_msg ft t \<lbrace>\<lambda>s :: det_state. P (domain_time s) (scheduler_action s)\<rbrace>"
   assumes make_arch_fault_msg_domain_list_inv'[wp]:
     "\<And>P ft t. \<lbrace>\<lambda>s::det_state. P (domain_list s)\<rbrace> make_arch_fault_msg ft t \<lbrace>\<lambda>_ s. P (domain_list s)\<rbrace>"
-  assumes make_arch_fault_msg_domain_consumed_time_inv'[wp]:
-    "\<And>P ft t. \<lbrace>\<lambda>s::det_state. P (domain_time s)(consumed_time s)\<rbrace>
-         make_arch_fault_msg ft t \<lbrace>\<lambda>_ s. P (domain_time s)(consumed_time s)\<rbrace>"
-  assumes make_arch_fault_msg_domain_consumed_inv'[wp]:
-    "\<And>P ft t. \<lbrace>\<lambda>s::det_state. P (domain_time s)(consumed_time s)\<rbrace>
-             make_arch_fault_msg ft t \<lbrace>\<lambda>_ s. P (domain_time s)(consumed_time s)\<rbrace>"
-  assumes arch_post_cap_deletion_domain_time_inv'[wp]:
-    "\<And>P ft. \<lbrace>\<lambda>s::det_state. P (domain_time s)\<rbrace> arch_post_cap_deletion ft \<lbrace>\<lambda>_ s. P (domain_time s)\<rbrace>"
+  assumes arch_post_cap_deletion_domain_time_scheduler_action_inv'[wp]:
+    "\<And>P ft. arch_post_cap_deletion ft \<lbrace>\<lambda>s :: det_state. P (domain_time s) (scheduler_action s)\<rbrace>"
   assumes arch_post_cap_deletion_domain_list_inv'[wp]:
     "\<And>P ft. \<lbrace>\<lambda>s::det_state. P (domain_list s)\<rbrace> arch_post_cap_deletion ft \<lbrace>\<lambda>_ s. P (domain_list s)\<rbrace>"
   assumes arch_invoke_irq_handler_domain_list_inv'[wp]:
     "\<And>P i. arch_invoke_irq_handler i \<lbrace>\<lambda>s::det_state. P (domain_list s)\<rbrace>"
-  assumes arch_invoke_irq_handler_domain_time_inv'[wp]:
-    "\<And>P i. arch_invoke_irq_handler i \<lbrace>\<lambda>s::det_state. P (domain_time s)\<rbrace>"
+  assumes arch_invoke_irq_handler_domain_time_scheduler_action_inv'[wp]:
+    "\<And>P i. arch_invoke_irq_handler i \<lbrace>\<lambda>s::det_state. P (domain_time s) (scheduler_action s)\<rbrace>"
 
 crunches update_restart_pc
   for domain_list[wp]: "\<lambda>s. P (domain_list s)"
@@ -117,27 +110,25 @@ crunches update_restart_pc
 locale DetSchedDomainTime_AI_2 = DetSchedDomainTime_AI +
   assumes handle_hypervisor_fault_domain_list_inv'[wp]:
     "\<And>P t f. \<lbrace>\<lambda>s::det_state. P (domain_list s)\<rbrace> handle_hypervisor_fault t f \<lbrace>\<lambda>_ s. P (domain_list s)\<rbrace>"
-  assumes handle_hypervisor_fault_domain_time_inv'[wp]:
-    "\<And>P t f. \<lbrace>\<lambda>s::det_state. P (domain_time s)\<rbrace> handle_hypervisor_fault t f \<lbrace>\<lambda>_ s. P (domain_time s)\<rbrace>"
+  assumes handle_hypervisor_fault_domain_time_scheduler_action_inv'[wp]:
+    "\<And>P t f. handle_hypervisor_fault t f \<lbrace>\<lambda>s :: det_state. P (domain_time s) (scheduler_action s)\<rbrace>"
   assumes arch_perform_invocation_domain_list_inv'[wp]:
     "\<And>P i. \<lbrace>\<lambda>s::det_state. P (domain_list s)\<rbrace> arch_perform_invocation i \<lbrace>\<lambda>_ s. P (domain_list s)\<rbrace>"
-  assumes arch_perform_invocation_domain_time_inv'[wp]:
-    "\<And>P i. \<lbrace>\<lambda>s::det_state. P (domain_time s)\<rbrace> arch_perform_invocation i \<lbrace>\<lambda>_ s. P (domain_time s)\<rbrace>"
+  assumes arch_perform_invocation_domain_time_scheduler_action_inv'[wp]:
+    "\<And>P i. arch_perform_invocation i \<lbrace>\<lambda>s :: det_state. P (domain_time s) (scheduler_action s)\<rbrace>"
   assumes handle_interrupt_valid_domain_time:
     "\<And>i.
       \<lbrace>\<lambda>s :: det_state. 0 < domain_time s \<rbrace>
         handle_interrupt i
       \<lbrace>\<lambda>rv s.  domain_time s = 0 \<longrightarrow> scheduler_action s = choose_new_thread \<rbrace>"
-  assumes handle_reserved_irq_some_time_inv'[wp]:
-    "\<And>P irq. \<lbrace>\<lambda>s::det_state. P (domain_time s)\<rbrace> handle_reserved_irq irq \<lbrace>\<lambda>_ s. P (domain_time s)\<rbrace>"
+  assumes handle_reserved_irq_some_time_scheduler_action_inv'[wp]:
+    "\<And>P irq. handle_reserved_irq irq \<lbrace>\<lambda>s :: det_state. P (domain_time s) (scheduler_action s)\<rbrace>"
   assumes handle_reserved_irq_domain_list_inv'[wp]:
     "\<And>P irq. \<lbrace>\<lambda>s::det_state. P (domain_list s)\<rbrace> handle_reserved_irq irq \<lbrace>\<lambda>_ s. P (domain_list s)\<rbrace>"
   assumes arch_mask_irq_signal_domain_list_inv'[wp]:
     "\<And>P irq. arch_mask_irq_signal irq \<lbrace>\<lambda>s::det_state. P (domain_list s)\<rbrace>"
-  assumes arch_mask_irq_signal_domain_time_inv'[wp]:
-    "\<And>P irq. arch_mask_irq_signal irq \<lbrace>\<lambda>s::det_state. P (domain_time s)\<rbrace>"
-
-crunch (empty_fail) empty_fail[wp]: commit_domain_time
+  assumes arch_mask_irq_signal_domain_time_scheduler_action_inv'[wp]:
+    "\<And>P irq. arch_mask_irq_signal irq \<lbrace>\<lambda>s::det_state. P (domain_time s) (scheduler_action s)\<rbrace>"
 
 context DetSchedDomainTime_AI begin
 
@@ -167,9 +158,6 @@ lemma rec_del_domain_list[wp]:
 
 crunch domain_list_inv[wp]: cap_delete, activate_thread "\<lambda>s::det_state. P (domain_list s)"
   (wp: hoare_drop_imp)
-
-crunch domain_list_inv[wp]: possible_switch_to "\<lambda>s. P (domain_list s)"
-  (simp: get_tcb_obj_ref_def wp: hoare_vcg_if_lift2 hoare_drop_imp)
 
 crunches awaken
   for domain_list_inv[wp]: "\<lambda>s. P (domain_list s)"
@@ -268,7 +256,7 @@ crunches
 context DetSchedDomainTime_AI begin
 
 crunch domain_list_inv[wp]:
-  refill_budget_check,charge_budget, check_budget
+  refill_budget_check, charge_budget, check_budget
   "\<lambda>s::det_state. P (domain_list s)"
   (wp: crunch_wps check_cap_inv maybeM_inv simp: Let_def)
 
@@ -359,7 +347,7 @@ lemma handle_recv_domain_list_inv[wp]:
   by (rule_tac Q'="\<lambda>_ s. P (domain_list s)" in hoare_post_imps(1))  wpsimp+
 
 crunches
-  handle_yield, handle_call, handle_vm_fault, handle_hypervisor_fault
+  handle_yield, handle_call, handle_vm_fault, handle_hypervisor_fault, check_domain_time
   for domain_list_inv[wp]: "\<lambda>s::det_state. P (domain_list s)"
   (wp: crunch_wps simp: crunch_simps)
 
@@ -375,6 +363,10 @@ lemma handle_event_domain_list_inv[wp]:
       apply (case_tac syscall, simp_all add: handle_send_def whenE_def)
              apply wpsimp+
   done
+
+crunches preemption_path
+  for domain_list[wp]: "\<lambda>s::det_state. P (domain_list s)"
+  (wp: crunch_wps simp: crunch_simps)
 
 (* no one modifies domain_list - supplied at compile time *)
 lemma call_kernel_domain_list_inv_det_ext:
@@ -393,363 +385,354 @@ end
 
 section \<open>Preservation of domain time remaining\<close>
 
-crunch domain_time_inv[wp]: do_user_op "\<lambda>s. P (domain_time s)"
+definition dtime_bounded_2 where
+  "dtime_bounded_2 dt sa \<equiv> 0 = dt \<longrightarrow> sa = choose_new_thread"
+
+abbreviation dtime_bounded where
+  "dtime_bounded s \<equiv> dtime_bounded_2 (domain_time s) (scheduler_action s)"
+
+lemmas dtime_bounded_def = dtime_bounded_2_def
+
+lemma dtime_bounded_simp[simp]:
+  "dtime_bounded_2 dt (choose_new_thread)"
+  apply (clarsimp simp: dtime_bounded_2_def)
+  done
+
+lemma set_scheduler_action_dtime_bounded[wp]:
+  "\<lbrace>\<lambda>s. dtime_bounded_2 (domain_time s) sa \<rbrace> set_scheduler_action sa \<lbrace>\<lambda>_. dtime_bounded\<rbrace>"
+  unfolding set_scheduler_action_def
+  by wpsimp
+
+lemma set_scheduler_action_cdfgtime_bounded[wp]:
+  "\<lbrace>\<top>\<rbrace> reschedule_required \<lbrace>\<lambda>_. dtime_bounded\<rbrace>"
+  unfolding reschedule_required_def
+  apply (wpsimp wp: thread_get_wp hoare_vcg_if_lift2 is_schedulable_wp)
+  apply (clarsimp simp: dtime_bounded_def is_schedulable_bool_def' obj_at_def is_tcb_def
+                        pred_tcb_at_def)
+  done
+
+crunches  do_user_op
+  for domain_time_scheduler_action_inv[wp]:"\<lambda>s. P (domain_time s) (scheduler_action s)"
   (wp: select_wp)
 
-crunch domain_time_inv[wp]: schedule_tcb,tcb_release_remove "\<lambda>s. P (domain_time s)"
-  (wp: crunch_wps)
+crunches schedule_tcb, tcb_release_remove, set_thread_state, store_word_offs
+  for dtime_bounded[wp]: dtime_bounded
+  (wp: crunch_wps simp: crunch_simps)
 
-crunch domain_time_inv[wp]: set_thread_state,store_word_offs "\<lambda>s. P (domain_time s)"
-  (wp: crunch_wps)
+crunches set_mrs
+  for domain_time_scheduler_action_inv[wp]: "\<lambda>s. P (domain_time s) (scheduler_action s)"
+  (wp: crunch_wps simp: crunch_simps)
 
-lemma set_mrs_domain_time_inv[wp]:
-  "\<lbrace>\<lambda>s. P (domain_time s)\<rbrace> set_mrs param_a param_b param_c \<lbrace>\<lambda>_ s. P (domain_time s)\<rbrace>"
-  by (wpsimp simp: set_mrs_def zipWithM_x_mapM split_del: if_split wp: mapM_wp')
-
-crunch domain_time_inv[wp]: complete_yield_to "\<lambda>s. P (domain_time s)"
+crunches complete_yield_to
+  for domain_time_scheduler_action_inv[wp]:"\<lambda>s. P (domain_time s) (scheduler_action s)"
   (wp: crunch_wps maybeM_inv)
 
 context DetSchedDomainTime_AI begin
 
-crunch domain_time_inv[wp]:
-  get_cap, activate_thread, set_scheduler_action, tcb_sched_action
-  "\<lambda>s::det_state. P (domain_time s)" (wp: hoare_drop_imp)
+crunches get_cap, activate_thread, tcb_sched_action
+  for dtime_bounded[wp]: "\<lambda>s :: det_state. dtime_bounded s"
 
-crunch domain_time_inv[wp]: guarded_switch_to "\<lambda>s::det_state. P (domain_time s)"
+crunches guarded_switch_to, choose_thread
+  for domain_time_scheduler_action_inv[wp]: "\<lambda>s :: det_state. P (domain_time s) (scheduler_action s)"
   (wp: hoare_drop_imp whenE_inv)
 
-crunch domain_time_inv[wp]: choose_thread "\<lambda>s::det_state. P (domain_time s)"
-crunch domain_time_inv[wp]: sched_context_donate "\<lambda>s::det_state. P (domain_time s)"
+crunches maybe_donate_sc
+  for dtime_bounded[wp]: "\<lambda>s :: det_state. dtime_bounded s"
+  (wp: crunch_wps simp: crunch_simps)
 
-crunch domain_time_inv[wp]: reply_remove, maybe_donate_sc "\<lambda>s::det_state. P (domain_time s)"
-  (wp: hoare_drop_imps crunch_wps simp: crunch_simps)
+crunches update_sk_obj_ref
+  for dtime_bounded[wp]: "\<lambda>s :: det_state. dtime_bounded s"
+  (wp: crunch_wps simp: crunch_simps)
 
-crunch domain_time_inv[wp]: send_signal "\<lambda>s::det_state. P (domain_time s)"
+lemma reply_unlink_tcb_dtime_bounded[wp]:
+  "reply_unlink_tcb t r \<lbrace>\<lambda>s :: det_state. dtime_bounded s\<rbrace>"
+  apply (clarsimp simp: reply_unlink_tcb_def)
+  apply (wpsimp wp: gts_wp hoare_drop_imps)
+  done
+
+crunches reply_remove
+  for dtime_bounded[wp]: "\<lambda>s :: det_state. dtime_bounded s"
+  (wp: hoare_drop_imps crunch_wps simp: crunch_simps update_sk_obj_ref_def)
+
+lemma possible_switch_to_dtime_bounded[wp]:
+  "possible_switch_to tcb_ptr \<lbrace>\<lambda>s :: det_state. dtime_bounded s\<rbrace>"
+  apply (clarsimp simp: possible_switch_to_def)
+  apply (wpsimp wp: thread_get_inv | wp (once) hoare_drop_imp)+
+  apply (clarsimp simp: obj_at_def dtime_bounded_def not_in_release_q_def)
+  done
+
+crunches send_signal
+  for dtime_bounded[wp]: "\<lambda>s :: det_state. dtime_bounded s"
   (wp: hoare_drop_imps mapM_x_wp_inv maybeM_inv select_wp simp: crunch_simps unless_def)
 
-crunch domain_time_inv[wp]:
-  cap_swap_for_delete, empty_slot, get_object, get_cap, tcb_sched_action
-  "\<lambda>s::det_state. P (domain_time s)"
+crunches cap_swap_for_delete, empty_slot, get_object, get_cap, tcb_sched_action
+  for domain_time_scheduler_act_inv[wp]: "\<lambda>s :: det_state. P (domain_time s) (scheduler_action s)"
 
-crunch domain_time_inv[wp]: sched_context_unbind_tcb "\<lambda>s. P (domain_time s)" (wp: hoare_drop_imp)
+crunches sched_context_unbind_tcb
+  for dtime_bounded[wp]: "\<lambda>s :: det_state. dtime_bounded s"
+  (wp: hoare_drop_imp simp: crunch_simps)
 
-crunch domain_time_inv[wp]: finalise_cap "\<lambda>s::det_state. P (domain_time s)"
-  (wp: crunch_wps hoare_drop_imps hoare_unless_wp select_inv mapM_wp
-       subset_refl if_fun_split maybeM_inv simp: crunch_simps ignore: tcb_sched_action)
+crunches finalise_cap
+  for dtime_bounded[wp]: "\<lambda>s :: det_state. dtime_bounded s"
+  (wp: crunch_wps maybeM_inv)
 
-lemma rec_del_domain_time[wp]:
-  "\<lbrace>\<lambda>s::det_state. P (domain_time s)\<rbrace> rec_del call \<lbrace>\<lambda>rv s. P (domain_time s)\<rbrace>"
-  by (wp rec_del_preservation preemption_point_inv' | simp)+
+lemma preemption_point_dtime_bounded[wp]:
+  "\<lbrace>dtime_bounded\<rbrace> preemption_point \<lbrace>\<lambda>_ s :: det_state. dtime_bounded s\<rbrace>, -"
+  apply (clarsimp simp: preemption_point_def)
+  apply (clarsimp simp: validE_R_def)
+  apply (rule hoare_seq_ext_skipE, wpsimp)
+  apply (clarsimp simp: validE_R_def[symmetric])
+  apply (rule OR_choiceE_E_weak_wp)
+  apply (rule alternativeE_R_wp[where P=Q and P'=Q for Q, simplified pred_conj_def, simplified]
+         ; (solves wpsimp)?)
+  apply (clarsimp simp: validE_R_def)
+  apply (rule hoare_seq_ext_skipE, wpsimp)
+  apply (rule_tac B="\<top>\<top>" in seqE)
+   apply wpsimp
+  apply (rule hoare_seq_ext_skipE, wpsimp)
+  apply wpsimp
+  apply (clarsimp simp: dtime_bounded_def is_cur_domain_expired_def num_domains_def)
+  done
 
-crunch domain_time_inv[wp]:
-  cap_delete, activate_thread, lookup_cap_and_slot
-  "\<lambda>s::det_state. P (domain_time s)"
+lemma rec_del_dtime_bounded[wp]:
+  "\<lbrace>dtime_bounded\<rbrace> rec_del call \<lbrace>\<lambda>_ s :: det_state. dtime_bounded s\<rbrace>, -"
+  by (wpsimp wp: rec_del_preservationE)
 
-end
+lemma cap_delete_dtime_bounded[wp]:
+  "\<lbrace>dtime_bounded\<rbrace> cap_delete slot \<lbrace>\<lambda>_ s :: det_state. dtime_bounded s\<rbrace>, -"
+  by (wpsimp simp: cap_delete_def)
 
-crunch domain_time_inv[wp]: cap_insert "\<lambda>s::det_state. P (domain_time s)"
+crunches cap_insert
+  for domain_time_scheduler_action_inv[wp]: "\<lambda>s :: det_state. P (domain_time s) (scheduler_action s)"
   (wp: hoare_drop_imps)
 
-crunch domain_time_inv[wp]: set_extra_badge "\<lambda>s. P (domain_time s)"
+crunches set_extra_badge
+  for domain_time_scheduler_action_inv[wp]: "\<lambda>s. P (domain_time s) (scheduler_action s)"
 
-crunch domain_time_inv[wp]: postpone,reply_push "\<lambda>s::det_state. P (domain_time s)"
-  (wp: hoare_drop_imp mapM_wp' hoare_vcg_if_lift)
+crunches sched_context_donate, bind_sc_reply, set_reply_obj_ref, set_thread_state, reply_push
+  for dtime_bounded[wp]: "\<lambda>s :: det_state. dtime_bounded s"
+  (wp: hoare_drop_imp mapM_wp' hoare_vcg_if_lift simp: crunch_simps)
 
-context DetSchedDomainTime_AI begin
-
-crunch domain_time_inv[wp]: do_ipc_transfer "\<lambda>s::det_state. P (domain_time s)"
+crunches do_ipc_transfer
+  for domain_time_scheduler_action_inv[wp]: "\<lambda>s :: det_state. P (domain_time s) (scheduler_action s)"
   (wp: crunch_wps transfer_caps_loop_pres simp: zipWithM_x_mapM ignore: transfer_caps_loop)
 
-crunch domain_time_inv[wp]: send_ipc "\<lambda>s::det_state. P (domain_time s)"
-  (wp: mapM_wp hoare_drop_imps maybeM_inv simp: crunch_simps ignore:copy_mrs sched_context_donate)
+crunches handle_fault
+  for dtime_bounded[wp]: "\<lambda>s :: det_state. dtime_bounded s"
+  (wp: mapM_wp hoare_drop_imps maybeM_inv simp: crunch_simps ignore: copy_mrs sched_context_donate)
 
-crunch domain_time_inv[wp]: send_fault_ipc "\<lambda>s::det_state. P (domain_time s)"
+crunches reply_from_kernel, create_cap, retype_region
+  for domain_time_scheduler_action_inv[wp]: "\<lambda>s :: det_state. P (domain_time s) (scheduler_action s)"
 
-crunch domain_time_inv[wp]: handle_fault "\<lambda>s::det_state. P (domain_time s)"
-  (wp: mapM_wp hoare_drop_imps maybeM_inv hoare_unless_wp simp: crunch_simps ignore:copy_mrs)
+crunches do_reply_transfer
+  for dtime_bounded[wp]:"\<lambda>s::det_state. dtime_bounded s"
+  (wp: hoare_drop_imps)
 
-crunch domain_time_inv[wp]: reply_from_kernel, create_cap, retype_region
-  "\<lambda>s::det_state. P (domain_time s)"
+crunches delete_objects
+  for domain_time_scheduler_action_inv[wp]: "\<lambda>s :: det_state. P (domain_time s) (scheduler_action s)"
+  (simp: detype_def)
 
-crunch domain_time_inv[wp]: do_reply_transfer "\<lambda>s::det_state. P (domain_time s)"
-  (wp: hoare_drop_imps maybeM_inv mapM_wp)
-end
-
-crunch domain_time_inv[wp]: delete_objects "\<lambda>s :: det_state. P (domain_time s)"
-  (wp: crunch_wps
-   simp: detype_def wrap_ext_det_ext_ext_def cap_insert_ext_def
-   ignore: freeMemory)
-
-crunch domain_time_inv[wp]: preemption_point "\<lambda>s::det_state. P (domain_time s)"
-  (wp: select_inv OR_choiceE_weak_wp crunch_wps ignore: OR_choiceE ignore_del: preemption_point)
-
-crunch domain_time_inv[wp]: reset_untyped_cap "\<lambda>s::det_state. P (domain_time s)"
-  (wp: crunch_wps hoare_unless_wp mapME_x_inv_wp select_inv
-   simp: crunch_simps)
+lemma reset_untyped_cap_dtime_bounded[wp]:
+  "\<lbrace>dtime_bounded\<rbrace> reset_untyped_cap src_slot \<lbrace>\<lambda>_ s::det_state. dtime_bounded s\<rbrace>, -"
+  (is "\<lbrace>?pre\<rbrace> _ \<lbrace>_\<rbrace>, -")
+  apply (clarsimp simp: reset_untyped_cap_def)
+  apply (clarsimp simp: validE_R_def)
+  apply (rule hoare_seq_ext_skipE, wpsimp)
+  apply clarsimp
+  apply (intro conjI impI; (solves wpsimp)?)
+  apply (rule_tac Q="?pre" in hoare_weaken_preE[rotated], simp)
+  apply (rule hoare_seq_ext_skipE, wpsimp)
+  apply (rule_tac Q="\<lambda>_ . ?pre" and E="\<top>\<top>"in hoare_post_impErr; simp)
+  apply (wpsimp wp: mapME_x_wp_inv')
+  done
 
 crunches sched_context_bind_tcb, restart
-  for domain_time_inv[wp]: "\<lambda>s::det_state. P (domain_time s)"
-  (wp: hoare_drop_imp maybeM_inv)
+  for dtime_bounded[wp]: "\<lambda>s :: det_state. dtime_bounded s"
+  (wp: hoare_drop_imp maybeM_inv simp: crunch_simps)
 
 crunches refill_update, refill_new
-  for domain_time_inv[wp]: "\<lambda>s. P (domain_time s)"
+  for domain_time_scheduler_action_inv[wp]: "\<lambda>s. P (domain_time s) (scheduler_action s)"
   (wp: crunch_wps)
 
-crunches set_extra_badge, schedule_tcb
-  for domain_consumed_time_inv[wp]: "\<lambda>s. P (domain_time s)(consumed_time s)"
-  (wp: crunch_wps)
+crunches refill_budget_check, charge_budget, refill_budget_check_round_robin
+  for dtime_bounded[wp]: "\<lambda>s :: det_state. dtime_bounded s"
+  (wp: crunch_wps check_cap_inv maybeM_inv simp: Let_def crunch_simps)
 
-crunches cap_insert, set_thread_state, postpone, reply_push
-  for domain_consumed_time_inv[wp]: "\<lambda>s::det_state. P (domain_time s)(consumed_time s)"
-  (wp: hoare_drop_imps mapM_wp' hoare_vcg_if_lift)
-
-context DetSchedDomainTime_AI begin
-
-crunch domain_time_inv[wp]:
-  refill_budget_check,charge_budget,refill_budget_check_round_robin
-  "\<lambda>s::det_state. P (domain_time s)"
-  (wp: crunch_wps check_cap_inv maybeM_inv simp: Let_def)
-
-crunch domain_time_inv[wp]: invoke_untyped "\<lambda>s::det_state. P (domain_time s)"
-  (wp: crunch_wps
-    simp: crunch_simps mapM_x_defsym)
-
-crunch domain_time_inv[wp]: invoke_tcb "\<lambda>s::det_state. P (domain_time s)"
-  (wp: crunch_wps check_cap_inv
-    simp: crunch_simps)
-
-crunch domain_time_inv[wp]:
-  invoke_domain, invoke_irq_control,invoke_irq_handler
-  "\<lambda>s::det_state. P (domain_time s)"
-  (wp: crunch_wps check_cap_inv maybeM_inv)
-
-
-crunch domain_time_inv[wp]: invoke_sched_context "\<lambda>s::det_state. P (domain_time s)"
-  (wp: crunch_wps check_cap_inv maybeM_inv
-    simp: crunch_simps)
-
-lemma commit_domain_time_domain_time:
-  "\<lbrace>\<lambda>s. P (if domain_time s < consumed_time s then 0 else domain_time s - consumed_time s)\<rbrace>
-      commit_domain_time \<lbrace>\<lambda>_ s. P (domain_time s)\<rbrace>"
-  by (wpsimp simp: commit_domain_time_def)
-
-crunch consumed_time_inv[wp]: set_thread_state,store_word_offs "\<lambda>s::det_state. P (consumed_time s)"
-  (wp: crunch_wps dxo_wp_weak)
-
-crunch domain_time_consumed_time[wp]: refill_budget_check, refill_budget_check_round_robin
-  "\<lambda>s::det_state. P (domain_time s)(consumed_time s)"
-  (wp: crunch_wps check_cap_inv maybeM_inv dxo_wp_weak
-   simp: zipWithM_x_mapM Let_def)
-
-crunch domain_time_consumed_time[wp]: do_ipc_transfer
-  "\<lambda>s::det_state. P (domain_time s)(consumed_time s)"
-  (wp: crunch_wps transfer_caps_loop_pres simp: zipWithM_x_mapM ignore: transfer_caps_loop)
-
-crunch domain_time_consumed_time[wp]: end_timeslice
-  "\<lambda>s::det_state. P (domain_time s)(consumed_time s)"
-  (wp: crunch_wps maybeM_inv simp: zipWithM_x_mapM ignore: do_reply_transfer)
-
-crunch valid_domain_list[wp]:
-  charge_budget,check_budget
-  "valid_domain_list :: det_state \<Rightarrow> _"
-  (wp: crunch_wps check_cap_inv mapM_wp' maybeM_inv simp: Let_def zipWithM_x_mapM)
-
-crunch domain_time_inv[wp]:
-  charge_budget,check_budget
-  "\<lambda>s::det_state. P (domain_time s)"
-  (wp: crunch_wps check_cap_inv mapM_wp' maybeM_inv simp: Let_def zipWithM_x_mapM)
-
-lemma charge_budget_domain_time_consumed_time:
-   "\<lbrace>\<lambda>s::det_state. P (domain_time s) 0 \<rbrace>
-    charge_budget consumed canTimeout
-    \<lbrace>\<lambda>_ s. P (domain_time s) (consumed_time s)\<rbrace> "
-  by (wpsimp simp: charge_budget_def wp: assert_inv)
-
-lemma check_budget_domain_time_left[wp]:
-  "\<lbrace> valid_domain_list and (\<lambda>s. consumed_time s < domain_time s)\<rbrace>
-   check_budget
-   \<lbrace>\<lambda>_ s::det_state. 0 < domain_time s \<rbrace>"
-  by (wpsimp simp: check_budget_def word_gt_0)
-
-lemma check_budget_domain_consumed_time_gt[wp]:
-  "\<lbrace>\<lambda>s::det_state. consumed_time s < domain_time s\<rbrace> check_budget \<lbrace>\<lambda>_ s. consumed_time s  < domain_time s \<rbrace>"
-  by (wpsimp simp: check_budget_def word_gt_0
-               wp: charge_budget_domain_time_consumed_time)
-
-lemma commit_domain_time_domain_time_left:
-  "\<lbrace> valid_domain_list and (\<lambda>s. consumed_time s < domain_time s)\<rbrace>
-   commit_domain_time
-   \<lbrace>\<lambda>_ s. 0 < domain_time s \<rbrace>"
-  apply (wpsimp simp: commit_domain_time_def Let_def)
-  using word_gt_0 by fastforce
-
-lemma commit_time_domain_time_left[wp]:
-  "\<lbrace> valid_domain_list and (\<lambda>s. consumed_time s < domain_time s)\<rbrace>
-   commit_time
-   \<lbrace>\<lambda>_ s::det_state. 0 < domain_time s \<rbrace>"
-  by (wpsimp simp: commit_time_def num_domains_def
-               wp: commit_domain_time_domain_time_left hoare_drop_imp)
-
-lemma invoke_sched_control_configure_flags_domain_time_inv[wp]:
-  "\<lbrace>valid_domain_list and (\<lambda>s. consumed_time s < domain_time s)\<rbrace>
-      invoke_sched_control_configure_flags i \<lbrace>\<lambda>_ s::det_state. 0 < domain_time s \<rbrace>"
-  by (cases i)
-     (wpsimp simp: invoke_sched_control_configure_flags_def split_def word_gt_0 tcb_release_remove_def
-       split_del: if_split
-       wp: hoare_vcg_if_lift2 hoare_drop_imp hoare_vcg_conj_lift
-           commit_time_domain_time_left[simplified word_neq_0_conv[symmetric]]
-           check_budget_domain_time_left[simplified word_neq_0_conv[symmetric]])
-
-end
-
-crunch domain_time_inv[wp]: cap_move "\<lambda>s::det_state. P (domain_time s)"
-
-context DetSchedDomainTime_AI begin
-lemma cap_revoke_domain_time_inv[wp]:
-  "\<lbrace>(\<lambda>s :: det_state. P (domain_time s))\<rbrace> cap_revoke a \<lbrace>\<lambda>rv s. P (domain_time s)\<rbrace>"
-  apply (rule cap_revoke_preservation2)
-  apply (wp preemption_point_inv'|simp)+
+lemma invoke_untyped_dtime_bounded[wp]:
+  "\<lbrace>dtime_bounded\<rbrace> invoke_untyped ui \<lbrace>\<lambda>_ s::det_state. dtime_bounded s\<rbrace>, -"
+  apply (clarsimp simp: invoke_untyped_def)
+  apply (cases ui; simp)
+  apply (clarsimp simp: validE_R_def whenE_def)
+  apply (intro conjI impI)
+   apply (wpsimp wp: mapM_x_wp_inv reset_untyped_cap_dtime_bounded)+
   done
-end
 
-crunch domain_time_inv[wp]: cancel_badged_sends "\<lambda>s::det_state. P (domain_time s)"
-  (ignore: filterM clearMemory
-     simp: filterM_mapM crunch_simps
-       wp: crunch_wps)
+lemma install_tcb_frame_cap_dtime_bounded[wp]:
+  "\<lbrace>dtime_bounded\<rbrace> install_tcb_frame_cap target slot buffer \<lbrace>\<lambda>_ s :: det_state. dtime_bounded s\<rbrace>, -"
+  apply (clarsimp simp: install_tcb_frame_cap_def cap_delete_def)
+  apply (cases buffer; clarsimp)
+   apply wpsimp
+  apply (clarsimp simp: validE_R_def)
+  apply (rule hoare_seq_ext_skipE, wpsimp wp: check_cap_inv)+
+  apply wpsimp
+  done
+
+lemma install_tcb_cap_dtime_bounded[wp]:
+  "\<lbrace>dtime_bounded\<rbrace> install_tcb_cap target slot n buffer \<lbrace>\<lambda>_ s :: det_state. dtime_bounded s\<rbrace>, -"
+  apply (clarsimp simp: install_tcb_cap_def)
+  apply (wpsimp wp: check_cap_inv)
+  done
+
+crunches maybe_sched_context_unbind_tcb, maybe_sched_context_bind_tcb, set_priority, set_mcpriority,
+         bind_notification
+  for dtime_bounded[wp]: "\<lambda>s :: det_state. dtime_bounded s"
+  (wp: crunch_wps)
+
+lemma invoke_tcb_dtime_bounded[wp]:
+  "\<lbrace>dtime_bounded\<rbrace> invoke_tcb iv \<lbrace>\<lambda>_ (s::det_state). dtime_bounded s\<rbrace>, -"
+  supply if_split [split del]
+  apply (cases iv; (solves \<open>wpsimp wp: mapM_x_wp_inv hoare_drop_imps hoare_vcg_if_lift2\<close>)?)
+   apply (clarsimp simp: validE_R_def)
+   apply (rule hoare_seq_ext_skipE, wpsimp)+
+   apply (wpsimp wp: hoare_vcg_if_lift2 hoare_drop_imps mapM_x_wp_inv)
+  apply (rename_tac ntfnpt_opt)
+  apply (case_tac ntfnpt_opt; wpsimp)
+  done
+
+crunches invoke_domain, invoke_irq_control,invoke_irq_handler
+  for dtime_bounded[wp]: "\<lambda>s :: det_state. dtime_bounded s"
+  (wp: crunch_wps check_cap_inv maybeM_inv simp: crunch_simps)
+
+crunches invoke_sched_context
+  for dtime_bounded[wp]: "\<lambda>s::det_state. dtime_bounded s"
+  (wp: crunch_wps)
+
+crunches refill_budget_check, refill_budget_check_round_robin
+  for domain_time_scheduler_action[wp]: "\<lambda>s :: det_state. P (domain_time s) (scheduler_action s)"
+  (wp: crunch_wps)
+
+crunches charge_budget, check_budget_restart, commit_time
+  for dtime_bounded[wp]: "\<lambda>s :: det_state. dtime_bounded s"
+  (wp: crunch_wps mapM_wp')
+
+lemma invoke_sched_control_configure_flags_dtime_bounded[wp]:
+  "\<lbrace>valid_domain_list and dtime_bounded\<rbrace>
+   invoke_sched_control_configure_flags i
+   \<lbrace>\<lambda>_ s :: det_state. dtime_bounded s\<rbrace>"
+  by (cases i; clarsimp)
+     (wpsimp simp: invoke_sched_control_configure_flags_def split_def word_gt_0
+                   tcb_release_remove_def
+        split_del: if_split
+               wp: hoare_vcg_if_lift2 hoare_drop_imp hoare_vcg_conj_lift)+
+
+crunches cap_move
+  for domain_time_scheduler_action_inv[wp]: "\<lambda>s :: det_state. P (domain_time s) (scheduler_action s)"
+
+lemma cap_revoke_dtime_bounded[wp]:
+  "\<lbrace>dtime_bounded\<rbrace> cap_revoke slot \<lbrace>\<lambda>_ s::det_state. dtime_bounded s\<rbrace>, -"
+  by (wpsimp wp: cap_revoke_preservationE)
+
+crunches cancel_badged_sends
+  for dtime_bounded[wp]: "\<lambda>s :: det_state. dtime_bounded s"
+
+end
 
 context DetSchedDomainTime_AI_2 begin
 
-lemma invoke_cnode_domain_time_inv[wp]:
-  "\<lbrace>\<lambda>s :: det_state. P (domain_time s)\<rbrace>
-     invoke_cnode i
-   \<lbrace>\<lambda>rv s. P (domain_time s) \<rbrace>"
-  apply (rule hoare_pre)
-   apply (wp crunch_wps cap_move_src_slot_Null hoare_drop_imps hoare_vcg_all_lift
-          | wpc | simp add: invoke_cnode_def crunch_simps split del: if_split)+
+lemma invoke_cnode_dtime_bounded[wp]:
+  "\<lbrace>dtime_bounded\<rbrace> invoke_cnode i \<lbrace>\<lambda>_ s::det_state. dtime_bounded s\<rbrace>, -"
+  apply (clarsimp simp: invoke_cnode_def cap_delete_def)
+  apply (cases i; clarsimp)
+       apply (wpsimp | intro conjI impI)+
   done
 
-lemma perform_invocation_domain_time_inv:
-  "\<lbrace>valid_domain_list and (\<lambda>s. consumed_time s < domain_time s)\<rbrace>
-      perform_invocation block call can_donate i \<lbrace>\<lambda>_ s::det_state. 0 < domain_time s \<rbrace>"
-  by (cases i; wpsimp; clarsimp simp: word_gt_0)
+lemma perfom_invocation_dtime_bounded[wp]:
+  "\<lbrace>dtime_bounded and valid_domain_list\<rbrace>
+   perform_invocation block call can_donate iv
+   \<lbrace>\<lambda>_ s::det_state. dtime_bounded s\<rbrace>, -"
+  by (cases iv; wpsimp)
 
-lemma handle_invocation_domain_time_inv[wp]:
-  "\<lbrace>valid_domain_list and (\<lambda>s. consumed_time s < domain_time s)\<rbrace>
-     handle_invocation calling blocking can_donate first_phase cptr
-   \<lbrace>\<lambda>_ s::det_state. 0 < domain_time s \<rbrace>"
-  by (wpsimp simp: handle_invocation_def
-      wp: syscall_valid crunch_wps perform_invocation_domain_time_inv)
-     (clarsimp simp: word_gt_0)
+lemma handle_invocation_dtime_bounded[wp]:
+  "\<lbrace>dtime_bounded and valid_domain_list\<rbrace>
+   handle_invocation calling blocking can_donate first_phase cptr
+   \<lbrace>\<lambda>_ s::det_state. dtime_bounded s\<rbrace>, -"
+  unfolding handle_invocation_def
+  by (wpsimp wp: syscall_valid hoare_drop_imps)
 
-crunch domain_time_inv[wp]: receive_ipc,lookup_reply "\<lambda>s::det_state. P (domain_time s)"
+crunches receive_ipc, lookup_reply, receive_signal, handle_interrupt, lookup_cap, handle_recv,
+         handle_yield, handle_vm_fault, handle_hypervisor_fault
+  for dtime_bounded[wp]: "\<lambda>s :: det_state. dtime_bounded s"
   (wp: crunch_wps simp: crunch_simps)
 
-crunch domain_time_inv[wp]: receive_signal "\<lambda>s::det_state. P (domain_time s)"
-  (wp: hoare_drop_imp hoare_vcg_if_lift2)
+lemma handle_call_dtime_bounded[wp]:
+  "\<lbrace>valid_domain_list and dtime_bounded\<rbrace> handle_call \<lbrace>\<lambda>_ s :: det_state. dtime_bounded s \<rbrace>, -"
+  by (wpsimp simp: handle_call_def)
 
-lemma handle_recv_domain_time_inv[wp]:
-  "\<lbrace>\<lambda>s. P (domain_time s)\<rbrace>
-  handle_recv is_blocking can_reply \<lbrace>\<lambda>rv s::det_state. P (domain_time s)\<rbrace>"
-  apply (wpsimp simp: handle_recv_def Let_def whenE_def get_sk_obj_ref_def
-                split_del: if_split wp: hoare_drop_imps)
-  by (rule_tac Q'="\<lambda>_ s. P (domain_time s)" in hoare_post_imps(1))  wpsimp+
+lemma handle_send_dtime_bounded[wp]:
+  "\<lbrace>valid_domain_list and dtime_bounded\<rbrace> handle_send bl \<lbrace>\<lambda>_ s :: det_state. dtime_bounded s \<rbrace>, -"
+  by (wpsimp simp: handle_send_def)
 
+lemma check_domain_time_dtime_bounded[wp]:
+  "\<lbrace>\<top>\<rbrace> check_domain_time \<lbrace>\<lambda>_ s :: det_state. dtime_bounded s\<rbrace>"
+  apply (clarsimp simp: check_domain_time_def)
+  apply wpsimp
+  apply (clarsimp simp: dtime_bounded_def is_cur_domain_expired_def num_domains_def)
+  done
 
-crunch domain_time_inv[wp]: handle_yield, handle_vm_fault, handle_hypervisor_fault
-  "\<lambda>s::det_state. P (domain_time s)"
-  (wp: crunch_wps simp: crunch_simps)
-
-lemma handle_call_domain_time_inv[wp]:
-  "\<lbrace>valid_domain_list and (\<lambda>s. consumed_time s < domain_time s)\<rbrace>
-      handle_call \<lbrace>\<lambda>_ s::det_state. 0 < domain_time s \<rbrace>"
-  by (wpsimp simp: handle_call_def wp: handle_invocation_domain_time_inv)
-
-lemma check_budget_restart_domain_time_inv[wp]:
-  "\<lbrace>valid_domain_list and (\<lambda>s. consumed_time s < domain_time s)\<rbrace>
-      check_budget_restart \<lbrace>\<lambda>_ s::det_state. 0 < domain_time s \<rbrace>"
-  by (wpsimp simp: check_budget_restart_def)
-
-lemma check_budget_restart_domain_consumed_time_gt[wp]:
-  "\<lbrace>(\<lambda>s. consumed_time s < domain_time s)\<rbrace>
-      check_budget_restart \<lbrace>\<lambda>_ s::det_state. consumed_time s  < domain_time s \<rbrace>"
-  by (wpsimp simp: check_budget_restart_def)
-(*
-lemma update_time_stamp_domain_consumed_time_gt[wp]:
-  "\<lbrace>\<lambda>s. P (domain_time s)\<rbrace>
-      update_time_stamp \<lbrace>\<lambda>_ s. P (domain_time s)(consumed_time s) \<rbrace>"
-  apply (clarsimp simp: update_time_stamp_def)
-  apply (wpsimp simp: do_machine_op_def ARM.getCurrentTime_def)
-
-
-lemma handle_event_domain_time_inv:
-  "\<lbrace>valid_domain_list and (\<lambda>s. consumed_time s < domain_time s) and K (e \<noteq> Interrupt)\<rbrace>
-      handle_event e \<lbrace>\<lambda>_ s. 0 < domain_time s\<rbrace>"
-  apply (cases e, simp_all)
-      apply (rename_tac syscall)
-      apply (case_tac syscall, simp_all add: handle_send_def whenE_def)
-             apply (wpsimp split_del: if_split wp: hoare_vcg_if_lift2 hoare_drop_imp)+
-  apply (clarsimp simp: valid_domain_list_def)
-  using word_gt_0 by fastforce*)
+lemma handle_event_dtime_bounded[wp]:
+  "\<lbrace>valid_domain_list and dtime_bounded\<rbrace> handle_event e \<lbrace>\<lambda>_ s :: det_state. dtime_bounded s \<rbrace>, -"
+  apply (cases e; (solves \<open>wpsimp\<close>)?; simp)
+  apply (wpsimp wp: hoare_drop_imps)
+  done
 
 end
 
-lemma reschedule_required_valid_domain_time:
-  "\<lbrace> \<top> \<rbrace> reschedule_required
-   \<lbrace>\<lambda>x s. domain_time s = 0 \<longrightarrow> scheduler_action s = choose_new_thread\<rbrace>"
-  unfolding reschedule_required_def set_scheduler_action_def
-  by (wpsimp wp: hoare_vcg_imp_lift is_schedulable_wp simp: thread_get_def)
-
-crunch domain_time_inv[wp]: set_next_interrupt "\<lambda>s. P (domain_time s)"
+crunches set_next_interrupt
+  for domain_time_scheduler_action_inv[wp]: "\<lambda>s. P (domain_time s) (scheduler_action s)"
   (wp: hoare_drop_imps)
-
 
 context DetSchedDomainTime_AI begin
 
-lemma switch_sched_context_domain_time_left[wp]:
-  "\<lbrace>valid_domain_list and (\<lambda>s. consumed_time s < domain_time s)\<rbrace>
-   switch_sched_context
-   \<lbrace>\<lambda>_ s :: det_state. 0 < domain_time s\<rbrace>"
-  apply (wpsimp simp: switch_sched_context_def refill_unblock_check_defs
-                  wp: hoare_vcg_if_lift2 hoare_drop_imp whileLoop_wp' split_del: if_split)
-  apply (clarsimp simp: word_gt_0)
+crunches switch_sched_context, sc_and_timer
+  for domain_time_scheduler_action_inv[wp]: "\<lambda>s. P (domain_time s) (scheduler_action s)"
+  (wp: crunch_wps)
+
+lemma next_domain_domain_time_left[wp]:
+  "\<lbrace>valid_domain_list\<rbrace> next_domain \<lbrace>\<lambda>_ s. 0 < domain_time s \<rbrace>"
+  apply (clarsimp simp: next_domain_def)
+  apply (rule_tac B="\<lambda>_ s. 0 < domain_time s" in hoare_seq_ext)
+   apply (wpsimp wp: dxo_wp_weak)
+  apply wpsimp
+  apply (clarsimp simp: valid_domain_list_def all_set_conv_all_nth)
+  apply (erule_tac x="Suc (domain_index s) mod length (domain_list s)" in allE)
+  apply clarsimp
   done
 
-lemma sc_and_timer_domain_time_left[wp]:
-  "\<lbrace> valid_domain_list and (\<lambda>s. consumed_time s < domain_time s)\<rbrace>
-     sc_and_timer \<lbrace>\<lambda>_ s::det_state. 0 < domain_time s \<rbrace>"
-  by (wpsimp simp: sc_and_timer_def Let_def)
-(*
-lemma next_domain_domain_time_left[wp]:
-  "\<lbrace> valid_domain_list \<rbrace> next_domain \<lbrace>\<lambda>_ s. 0 < domain_time s \<rbrace>"
-  apply (wpsimp simp: next_domain_def Let_def)
-   apply (clarsimp simp: valid_domain_list_def)
-   apply (simp add: all_set_conv_all_nth)
-   apply (erule_tac x="Suc (domain_index s) mod length (domain_list s)" in allE)
-   apply (clarsimp simp: \<mu>s_to_ms_def)
-
-
 lemma schedule_choose_new_thread_domain_time_left[wp]:
-  "\<lbrace> valid_domain_list \<rbrace>
+  "\<lbrace>valid_domain_list\<rbrace>
    schedule_choose_new_thread
-   \<lbrace>\<lambda>_ s. 0 < domain_time s \<rbrace>"
+   \<lbrace>\<lambda>_ s :: det_state. 0 < domain_time s \<rbrace>"
   unfolding schedule_choose_new_thread_def
   by (wpsimp simp: word_gt_0)
 
-crunch valid_domain_list: schedule_choose_new_thread valid_domain_list
-
-crunch etcb_at[wp]: tcb_sched_action "etcb_at P t"
+crunches awaken
+  for dtime_bounded[wp]: "\<lambda>s :: det_state. dtime_bounded s"
+  (wp: crunch_wps)
 
 lemma schedule_domain_time_left:
-  "\<lbrace>valid_domain_list and (\<lambda>s. domain_time s = 0 \<longrightarrow> scheduler_action s = choose_new_thread) \<rbrace>
+  "\<lbrace>valid_domain_list and dtime_bounded\<rbrace>
    schedule
-   \<lbrace>\<lambda>_ s. 0 < domain_time s \<rbrace>" (is "\<lbrace>?P\<rbrace> _ \<lbrace>\<lambda>_ . ?Q\<rbrace>")
+   \<lbrace>\<lambda>_ s :: det_state. 0 < domain_time s \<rbrace>" (is "\<lbrace>?P\<rbrace> _ \<lbrace>_\<rbrace>")
   supply word_neq_0_conv[simp]
   apply (simp add: schedule_def)
-  apply (wp|wpc)+
-(*           apply (wp hoare_drop_imps)[1]
-          apply (wpsimp wp: gts_wp hoare_drop_imps simp: is_schedulable_def)+
-  done*)
-*)
+  apply (rule_tac B="\<lambda>_. ?P" in hoare_seq_ext[rotated])
+   apply wpsimp
+  apply (intro hoare_seq_ext[OF _ gets_sp]
+               hoare_seq_ext[OF _ is_schedulable_sp])
+  apply (wpsimp wp: hoare_drop_imps)
+  apply (fastforce simp: dtime_bounded_def)
+  done
+
 end
 
 (* FIXME: move to where hoare_drop_imp is, add E/R variants etc *)
@@ -758,29 +741,29 @@ lemma hoare_false_imp:
   by (auto simp: valid_def)
 
 context DetSchedDomainTime_AI_2 begin
-(*
+
+crunches activate_thread
+  for domain_time_inv[wp]: "\<lambda>s :: det_state. P (domain_time s)"
+
+lemma preemption_path_dtime_bounded[wp]:
+  "\<lbrace>\<top>\<rbrace> preemption_path \<lbrace>\<lambda>_ s :: det_state. dtime_bounded s\<rbrace>"
+  apply (clarsimp simp: preemption_path_def)
+  apply (wpsimp wp: check_domain_time_dtime_bounded is_schedulable_wp hoare_drop_imps
+              simp: is_schedulable_bool_def')
+  done
+
 lemma call_kernel_domain_time_inv_det_ext:
-  "\<lbrace> (\<lambda>s. 0 < domain_time s) and valid_domain_list and (\<lambda>s. e \<noteq> Interrupt \<longrightarrow> ct_running s) \<rbrace>
-   (call_kernel e) :: (unit,det_ext) s_monad
-   \<lbrace>\<lambda>_ s. 0 < domain_time s \<rbrace>"
+  "\<lbrace>(\<lambda>s. 0 < domain_time s) and valid_domain_list and (\<lambda>s. e \<noteq> Interrupt \<longrightarrow> ct_running s)\<rbrace>
+   call_kernel e
+   \<lbrace>\<lambda>_ s :: det_state. 0 < domain_time s \<rbrace>"
   unfolding call_kernel_def
-  apply (case_tac "e = Interrupt")
-   apply simp
-   apply (rule hoare_pre)
-   apply ((wp schedule_domain_time_left handle_interrupt_valid_domain_time
-           | wpc | simp)+)[1]
-   apply (rule_tac Q="\<lambda>_ s. 0 < domain_time s \<and> valid_domain_list s" in hoare_strengthen_post)
-    apply wp
-   apply fastforce+
-  (* now non-interrupt case; may throw but does not touch domain_time in handle_event *)
-  apply (wp schedule_domain_time_left without_preemption_wp handle_interrupt_valid_domain_time)
-    apply (rule_tac Q="\<lambda>_ s. 0 < domain_time s \<and> valid_domain_list s" in hoare_post_imp)
-(*     apply fastforce
-    apply (wp handle_event_domain_time_inv)+
-   apply (rule_tac Q'="\<lambda>_ s. 0 < domain_time s" in hoare_post_imp_R)
-    apply (wp handle_event_domain_time_inv)
-   apply fastf orce+
-  done*) *)
+  apply (case_tac "e = Interrupt"; clarsimp)
+   subgoal by (wpsimp wp: schedule_domain_time_left | wp (once) hoare_drop_imp)+
+  apply (rule_tac B="\<lambda>_. valid_domain_list and dtime_bounded" in hoare_seq_ext[rotated])
+   apply (wpsimp simp: dtime_bounded_def)
+  apply (wp schedule_domain_time_left without_preemption_wp)
+  done
+
 end
 
 end
